checkpoint new plan, yet again
now hoare doubles reason about exec, not exec_recover.  no recovery program.

things seem fairly straightforward, with two exceptions:

1. we often end up with a hypothesis of the form (.. ==> crash) and
   a goal of the form (..something else.. ==> emp * crash).  need to
   figure out how to match them up automatically.  maybe we'll always
   have just one goal of this shape, so we can always try using it.
   doing it by hand seems to mostly work.

2. there's an unfortunate existential problem with [for_ok] that's not
   clear how to solve.  we have a goal of the form

     {{ fun done crash => .. *
        [[ {{ fun done' crash' => .. [[ done' = done ]] * .. }} p ]]
     }} p

   to solve this, we [eapply pimpl_pre], which is:

     Theorem pimpl_pre:
       forall pre pre' pr,
       (forall done crash, pre done crash ==> [{{pre'}} pr])
       -> (forall done crash, pre done crash ==> pre' done crash)
       -> {{pre}} pr.

   which creates an existential variable for [pre'] that should be
   a function of [done] and [crash], but the [cancel] separation
   logic automation has a hard time constructing such a term..

need to finish threading this new plan through Log.v, and then try
to prove idempotent recovery and state a theorem that involves only
final recovered states, and not the intermediate crash predicates
(which, unfortunately, exec now requires as an argument...)

src/Hoare.v
@@ -4,34 +4,42 @@ Require Import Pred.
 Set Implicit Arguments.
 
 
-(** ** Hoare triples *)
+(** ** Hoare logic *)
 
-Definition corr (pre: pred) (prog1 prog2: prog) :=
-  forall m m' out,
-  pre m ->
-  exec_recover m prog1 prog2 m' out ->
-  out = Finished.
+Definition corr2 (pre: donecond -> pred -> pred) (p: prog) :=
+  forall done crash m m' out,
+  pre done crash m ->
+  exec done crash m p m' out ->
+  out <> Failed.
 
+Notation "{{ pre }} p" := (corr2 pre%pred p)
+  (at level 0, p at level 60).
+
+(*
 Notation "{{ pre }} p1 >> p2" := (corr pre%pred p1 p2)
   (at level 0, p1 at level 60, p2 at level 60).
+*)
 
 Theorem pimpl_ok:
-  forall pre pre' pr rec,
-  {{pre'}} pr >> rec ->
-  (pre ==> pre') ->
-  {{pre}} pr >> rec.
+  forall pre pre' pr,
+  {{pre'}} pr ->
+  (forall done crash, pre done crash ==> pre' done crash) ->
+  {{pre}} pr.
 Proof.
-  firstorder.
+  unfold corr2; intros.
+  eapply H; eauto.
+  eapply H0.
+  eauto.
 Qed.
 
 Theorem pimpl_ok_cont :
-  forall pre pre' A (k : A -> _) x y rec,
-  {{pre'}} k y >> rec ->
-  (pre ==> pre') ->
-  (pre ==> exists F, F * [[x = y]]) ->
-  {{pre}} k x >> rec.
+  forall pre pre' A (k : A -> _) x y,
+  {{pre'}} k y ->
+  (forall done crash, pre done crash ==> pre' done crash) ->
+  (forall done crash, pre done crash ==> exists F, F * [[x = y]]) ->
+  {{pre}} k x.
 Proof.
-  unfold corr, pimpl; intros.
+  unfold corr2, pimpl; intros.
   edestruct H1; eauto.
   eapply sep_star_lift_l in H4; [|instantiate (1:=([x=y])%pred)].
   unfold lift in H4; rewrite H4 in *; eauto.
@@ -39,34 +47,40 @@ Proof.
 Qed.
 
 Theorem pimpl_pre:
-  forall pre pre' pr rec,
-  (pre ==> [{{pre'}} pr >> rec]) ->
-  (pre ==> pre') ->
-  {{pre}} pr >> rec.
+  forall pre pre' pr,
+  (forall done crash, pre done crash ==> [{{pre'}} pr])
+  -> (forall done crash, pre done crash ==> pre' done crash)
+  -> {{pre}} pr.
 Proof.
-  firstorder.
+  unfold corr2; intros.
+  eapply H; eauto.
+  eapply H0.
+  eauto.
 Qed.
 
 Theorem pre_false:
-  forall pre p1 p2,
-  (pre ==> [False]) ->
-  {{ pre }} p1 >> p2.
+  forall pre p,
+  (forall done crash, pre done crash ==> [False])
+  -> {{ pre }} p.
 Proof.
   firstorder.
 Qed.
 
 Theorem corr_exists:
-  forall T pre p rec,
-  (forall (a:T), {{ pre a }} p >> rec) ->
-  {{ exists a:T, pre a }} p >> rec.
+  forall T pre p,
+  (forall (a:T), {{ fun done crash => pre done crash a }} p)
+  -> {{ fun done crash => exists a:T, pre done crash a }} p.
 Proof.
-  firstorder.
+  unfold corr2; intros.
+  destruct H0.
+  eapply H; eauto.
 Qed.
 
-Theorem corr_forall: forall T pre p rec, {{ exists a:T, pre a }} p >> rec
-  -> forall (a:T), {{ pre a }} p >> rec.
+Theorem corr_forall: forall T pre p,
+  {{ fun done crash => exists a:T, pre done crash a }} p
+  -> forall (a:T), {{ fun done crash => pre done crash a }} p.
 Proof.
-  unfold corr; intros.
+  unfold corr2; intros.
   eapply H.
   exists a; eauto.
   eauto.
